Fix loop notations, add for loops

src/Util/Loop.v
@@ -1,7 +1,11 @@
 (** * Definition and Notations for [do { body }] *)
+Require Import Coq.ZArith.BinInt.
+Require Import Coq.micromega.Lia.
 Require Import Coq.omega.Omega.
+Require Import Crypto.Util.ZUtil.
 Require Import Crypto.Util.Notations.
 Require Import Crypto.Util.LetIn.
+Require Import Crypto.Util.Tactics.SpecializeBy.
 
 (* TODO: move *)
 Module CPSNotations.
@@ -11,7 +15,7 @@ Module CPSNotations.
   (* TODO: [cpscall] is a marker to get Coq to print code using this notation only when it was actually used *)
   Definition cpscall {R} (f:forall{T}(continuation:R->T),T) {T} (continuation:R->T)
     := @f T continuation.
-  Notation "x <- v ; C" := (cpscall v (fun x => C)) (at level 70, right associativity, format "'[v' x  <-  v ; '/' C ']'").
+  Notation "x' <- v ; C" := (cpscall v (fun x' => C)).
 
   (** A value of type [~>R] accepts a continuation that takes an
      argument of type [R].  It is meant to be used in [Definition] and
@@ -23,7 +27,7 @@ Module CPSNotations.
      [~> R] is universally quantified over the possible return types
      of the continuations that it can be applied to.
 *)
-  Notation "~> R" := (forall {T} (_:R->T), T) (at level 70).
+  Notation "~> R" := (forall {T} (_:R->T), T).
 
   (** The type [A ~> R] contains functions that takes an argument of
   type [A] and pass a value of type [R] to the continuation. Functions
@@ -31,12 +35,12 @@ Module CPSNotations.
   ~> B ~>C] -- the first form requires both arguments to be specified
   before its output can be CPS-bound, the latter must be bound once it
   is partially applied to one argument. *)
-  Notation "A ~> R" := (A -> ~>R) (at level 99).
-  
+  Notation "A ~> R" := (A -> ~>R).
+
   (* TODO: [cpsreturn] is a marker to get Coq to print loop notations before a [return] *)
   Definition cpsreturn {T} (x:T) := x.
   (** [return x] passes [x] to the continuation implicit in the previous notations. *)
-  Notation "'return' x" := (cpsreturn (fun {T} (continuation:_->T) => continuation x)) (at level 70, format "'return'  x").
+  Notation "'return' x" := (cpsreturn (fun {T} (continuation:_->T) => continuation x)).
 End CPSNotations.
 
 Section with_state.
@@ -104,7 +108,8 @@ Section with_state.
 
   Local Hint Extern 2 => omega.
 
-  Theorem loop_cps_wf_ind
+  (** TODO(andreser): Remove this if we don't need it *)
+  Theorem loop_cps_wf_ind_break
           (measure : state -> nat)
           (invariant : state -> Prop)
           T (P : T -> Prop) n v0 body rest
@@ -122,25 +127,203 @@ Section with_state.
     induction n as [|n IHn]; intros v0 rest Hinv Hbody Hmeasure; simpl; try omega.
     edestruct Hbody as [Hbody'|Hbody']; eauto.
   Qed.
+
+  Theorem loop_cps_wf_ind
+          (measure : state -> nat)
+          (invariant : state -> Prop)
+          T (P : T -> Prop) n v0 body rest
+    : invariant v0
+      -> (forall v continue,
+             invariant v
+             -> ((forall v', measure v' < measure v -> invariant v' -> P (continue v'))
+                 -> P (body v T continue rest)))
+      -> measure v0 < n
+      -> P (loop_cps n v0 body T rest).
+  Proof.
+    revert v0.
+    induction n as [|n IHn]; intros v0 Hinv Hbody Hmeasure; simpl; try omega.
+    eauto.
+  Qed.
 End with_state.
 
-(* N.B., Coq doesn't yet print this *)
+(** N.B. If the body is polymorphic (that is, if the type argument
+    shows up in the body), then we need to bind the name of the type
+    parameter somewhere in the notation for it to show up; we have a
+    separate notation for this case. *)
+(** TODO: When these notations are finalized, reserve them in Notations.v and moving the level and formatting rules there *)
+Notation "'loop' _{ fuel } ( state1 .. staten = initial ) 'labels' ( continue , break , @ T ) {{ body }} ; rest"
+  := (@loop_cps _ fuel initial
+                (fun state1 => .. (fun staten => id (fun T continue break => body)) .. )
+                _ (fun state1 => .. (fun staten => rest) .. ))
+       (at level 200, state1 binder, staten binder,
+        format "'[v  ' 'loop' _{ fuel }  ( state1 .. staten  =  initial )  'labels'  ( continue ,  break ,  @ T )  {{ '//' body ']' '//' }} ; '//' rest").
 Notation "'loop' _{ fuel } ( state1 .. staten = initial ) 'labels' ( continue , break ) {{ body }} ; rest"
   := (@loop_cps _ fuel initial
                 (fun state1 => .. (fun staten => id (fun T continue break => body)) .. )
                 _ (fun state1 => .. (fun staten => rest) .. ))
        (at level 200, state1 binder, staten binder,
         format "'[v  ' 'loop' _{ fuel }  ( state1 .. staten  =  initial )  'labels'  ( continue ,  break )  {{ '//' body ']' '//' }} ; '//' rest").
+Notation "'loop' _{ fuel } ( state1 .. staten = initial ) 'labels' ( continue ) {{ body }} ; rest"
+  := (@loop_cps _ fuel initial
+                (fun state1 => .. (fun staten => id (fun T continue _ => body)) .. )
+                _ (fun state1 => .. (fun staten => rest) .. ))
+       (at level 200, state1 binder, staten binder,
+        format "'[v  ' 'loop' _{ fuel }  ( state1 .. staten  =  initial )  'labels'  ( continue )  {{ '//' body ']' '//' }} ; '//' rest").
+
+Section with_for_state.
+  Import CPSNotations.
+  Context {state : Type}.
+
+  Section with_loop_params.
+    Context (test : Z -> Z -> bool) (i_final : Z) (upd_i : Z -> Z)
+            (body : state -> Z -> forall {T} (continue : state -> T) (break : state -> T), T).
+
+    (* we assume that [upd_i] is linear to compute the fuel *)
+    Definition for_cps (i0 : Z) (initial : state)
+      : ~> state
+      := fun T ret
+         => @loop_cps
+              (Z * state)
+              (S (S (Z.to_nat ((i_final - i0) / (upd_i 0%Z)))))
+              (i0, initial)
+              (fun '(i, st) T continue break
+               => if test i i_final
+                  then @body st i T
+                             (fun st' => continue (upd_i i, st')%Z)
+                             (fun st' => break (i, st'))
+                  else break (i, st))
+              T (fun '(i, st) => ret st).
+
+    Section lemmas.
+      Local Open Scope Z_scope.
+      Context (upd_linear : forall x, upd_i x = upd_i 0 + x)
+              (upd_signed : forall i0, test i0 i_final = true -> 0 < (i_final - i0) / (upd_i 0)).
+
+      (** TODO: Strengthen this to take into account the value of
+                  the loop counter at the end of the loop; based on
+                  [ForLoop.v], it should be something like [(finish -
+                  Z.sgn (finish - i0 + step - Z.sgn step) * (Z.abs
+                  (finish - i0 + step - Z.sgn step) mod Z.abs step) +
+                  step - Z.sgn step)] *)
+      Theorem for_cps_ind
+              (invariant : Z -> state -> Prop)
+              T (P : (*Z ->*) T -> Prop) i0 v0 rest
+        : invariant i0 v0
+          -> (forall i v continue,
+                 test i i_final = true
+                 -> (forall v, invariant (upd_i i) v -> P (continue v))
+                 -> invariant i v
+                 -> P (@body v i T continue rest))
+          -> (forall i v, test i i_final = false -> invariant i v -> P (rest v))
+          -> P (for_cps i0 v0 T rest).
+      Proof.
+        unfold for_cps, cpscall, cpsreturn.
+        intros Hinv IH Hrest.
+        eapply @loop_cps_wf_ind with (T:=T)
+                                       (invariant := fun '(i, s) => invariant i s)
+                                       (measure := fun '(i, s) => S (Z.to_nat ((i_final - i) / upd_i 0)));
+          [ assumption
+          |
+          | omega ].
+        intros [i st] continue Hinv' IH'.
+        destruct (test i i_final) eqn:Hi; [ | solve [ eauto ] ].
+        pose proof (upd_signed _ Hi) as upd_signed'.
+        assert (upd_i 0 <> 0)
+          by (intro H'; rewrite H' in upd_signed'; autorewrite with zsimplify in upd_signed';
+              omega).
+        specialize (IH i st (fun st' => continue (upd_i i, st')) Hi).
+        specialize (fun v pf => IH' (upd_i i, v) pf).
+        cbv beta iota in *.
+        specialize (fun pf v => IH' v pf).
+        rewrite upd_linear in IH'.
+        replace ((i_final - (upd_i 0 + i)) / upd_i 0)
+        with ((i_final - i) / upd_i 0 - 1)
+          in IH'
+          by (Z.div_mod_to_quot_rem; nia).
+        rewrite <- upd_linear, Z2Nat.inj_sub in IH' by omega.
+        assert ((Z.to_nat 0 < Z.to_nat ((i_final - i) / upd_i 0))%nat)
+          by (apply Z2Nat.inj_lt; omega).
+        change (Z.to_nat 0) with 0%nat in *.
+        change (Z.to_nat 1) with 1%nat in *.
+        auto with omega.
+      Qed.
+    End lemmas.
+  End with_loop_params.
+End with_for_state.
+
+Delimit Scope for_upd_scope with for_upd.
+Delimit Scope for_test_scope with for_test.
+Notation "i += k" := (Z.add i k) : for_upd_scope.
+Notation "i -= k" := (Z.sub i k) : for_upd_scope.
+Notation "i ++" := (i += 1)%for_upd : for_upd_scope.
+Notation "i --" := (i -= 1)%for_upd : for_upd_scope.
+Notation "<" := Z.ltb (at level 71) : for_test_scope.
+Notation ">" := Z.gtb (at level 71) : for_test_scope.
+Notation "<=" := Z.leb (at level 71) : for_test_scope.
+Notation ">=" := Z.geb (at level 71) : for_test_scope.
+Notation "≤" := Z.leb (at level 71) : for_test_scope.
+Notation "≥" := Z.geb (at level 71) : for_test_scope.
+Definition force_idZ (f : Z -> Z) (pf : f = id) {T} (v : T) := v.
+(** [lhs] and [cmp_expr] go at level 9 so that they bind more tightly
+    than application (so that [i (<)] sticks [i] in [lhs] and [(<)] in
+    [cmp_expr], rather than sticking [i (<)] in [lhs] and then
+    complaining about a missing value for [cmp_expr].  Unfortunately,
+    because the comparison operators need to be at level > 70 to not
+    conflict with their infix versions, putting [cmp_expr] at level 9
+    forces us to wrap parentheses around the comparison operator. *)
+(** TODO(andreser): If it's worth it, duplicate these notations for
+      each value of [cmp_expr] so that we don't need to wrap the
+      comparison operator in parentheses. *)
+(** TODO: When these notations are finalized, reserve them in Notations.v and moving the level and formatting rules there *)
+Notation "'for' ( i1 .. i2 = i0 ; lhs cmp_expr final ; upd_expr ) 'updating' ( state1 .. staten = initial ) 'labels' ( continue , break , @ T ) {{ body }} ; rest"
+  := (force_idZ
+        (fun i1 => .. (fun i2 => lhs) ..)
+        eq_refl
+        (@for_cps _ cmp_expr%for_test
+                  final
+                  (fun i1 => .. (fun i2 => upd_expr%for_upd) .. )
+                  (fun state1 => .. (fun staten => id (fun i1 => .. (fun i2 => id (fun T continue break => body)) .. )) .. )
+                  i0
+                  initial
+                  _ (fun state1 => .. (fun staten => rest) .. )))
+       (at level 200, state1 binder, staten binder, i1 binder, i2 binder, lhs at level 9, cmp_expr at level 9,
+        format "'[v  ' 'for'  ( i1 .. i2  =  i0 ;  lhs  cmp_expr  final ;  upd_expr )  'updating'  ( state1 .. staten  =  initial )  'labels'  ( continue ,  break ,  @ T )  {{ '//' body ']' '//' }} ; '//' rest").
+Notation "'for' ( i1 .. i2 = i0 ; lhs cmp_expr final ; upd_expr ) 'updating' ( state1 .. staten = initial ) 'labels' ( continue , break ) {{ body }} ; rest"
+  := (force_idZ
+        (fun i1 => .. (fun i2 => lhs) ..)
+        eq_refl
+        (@for_cps _ cmp_expr%for_test
+                  final
+                  (fun i1 => .. (fun i2 => upd_expr%for_upd) .. )
+                  (fun state1 => .. (fun staten => id (fun i1 => .. (fun i2 => id (fun T continue break => body)) .. )) .. )
+                  i0
+                  initial
+                  _ (fun state1 => .. (fun staten => rest) .. )))
+       (at level 200, state1 binder, staten binder, i1 binder, i2 binder, lhs at level 9, cmp_expr at level 9,
+        format "'[v  ' 'for'  ( i1 .. i2  =  i0 ;  lhs  cmp_expr  final ;  upd_expr )  'updating'  ( state1 .. staten  =  initial )  'labels'  ( continue ,  break )  {{ '//' body ']' '//' }} ; '//' rest").
+Notation "'for' ( i1 .. i2 = i0 ; lhs cmp_expr final ; upd_expr ) 'updating' ( state1 .. staten = initial ) 'labels' ( continue ) {{ body }} ; rest"
+  := (force_idZ
+        (fun i1 => .. (fun i2 => lhs) ..)
+        eq_refl
+        (@for_cps _ cmp_expr%for_test
+                  final
+                  (fun i1 => .. (fun i2 => upd_expr%for_upd) .. )
+                  (fun state1 => .. (fun staten => id (fun i1 => .. (fun i2 => id (fun T continue break => body)) .. )) .. )
+                  i0
+                  initial
+                  _ (fun state1 => .. (fun staten => rest) .. )))
+       (at level 200, state1 binder, staten binder, i1 binder, i2 binder, lhs at level 9, cmp_expr at level 9,
+        format "'[v  ' 'for'  ( i1 .. i2  =  i0 ;  lhs  cmp_expr  final ;  upd_expr )  'updating'  ( state1 .. staten  =  initial )  'labels'  ( continue )  {{ '//' body ']' '//' }} ; '//' rest").
 
 Section LoopTest.
   Import CPSNotations.
   Check loop _{ 10 } (x = 0) labels (continue, break) {{ continue (x + 1) }} ; x.
-                                                                                      
+
   Check
     loop _{ 1234 } ('(i, a) = (0, 0)) labels (continue, break)
     {{
         if i <? 10
-        then 
+        then
           continue (i + 1, a+1)
         else
           break (0, a)
@@ -155,27 +338,26 @@ Section LoopTest.
  Check loop _{ 10 } (x = 0) labels (continue, break) {{ continue (x + 1) }} ;
    return x.
 
- Check loop _{ 10 } (x = 0) labels (continue, break) {{ continue (x + 1) }} ; 
+ Check loop _{ 10 } (x = 0) labels (continue, break) {{ continue (x + 1) }} ;
    x <- f x;
    return x.
-  
-  (* TODO: the loop notation should print here. *)
-  Check loop _{ 10 } (x = 0) labels (continue, break) {{ x <- f x; continue (x) }} ; x.
 
-  (*
-  (* TODO LATER: something like these notations would be nice, desugaring to a [state := nat * T] *)
-  for ( i = s; i < f; i++) updating (P = zero) labels (continue, break)
+  Check loop _{ 10 } (x = 0) labels (continue, break) {{ x <- f x ; continue (x) }} ; x.
+
+
+  Axiom s F : Z.
+  Axiom zero : nat.
+  Check for ( i = s; i (<) F; i++) updating (P = zero) labels (continue, break)
   {{
       continue (P+P)
   }};
   P.
 
-  for ( i = s; i < f; i++) updating (P = zero) labels (continue)
+  Check for ( i = s; i (<) F; i++) updating (P = zero) labels (continue)
   {{
       continue (P+P)
   }};
   P.
-  *)
 End LoopTest.
 
 Require Import Crypto.Util.Tuple Crypto.Util.CPSUtil.
@@ -187,7 +369,7 @@ Section ScalarMult.
 
   (*
    table of xi*(32^i)*B
-        for 
+        for
         0 <= xi <= 8 (with sign flips, -8 <= xi <= 8)
         0 <= i <= 31
    *)
@@ -201,5 +383,5 @@ Section ScalarMult.
         continue (i', P_s)
     }};
   return P_s.
-  Print ScalarMultBase. (* TODO: the loop notation should print here *)
+  Print ScalarMultBase.
 End ScalarMult.
